Clap/eDSLState/Convert.lean
@@ -4,20 +4,31 @@ import Clap.Lang.Wheels
 
 namespace Clap
 
-structure Converts {p : ℕ} {α : Type}
-  (k : ℕ)
-  (conversion : α → Vector (ZMod p) k)
+class Sized (α : Type) where
+  size : ℕ
+
+notation "|" α "|" => Sized.size α
+
+class Convertible (p : ℕ) (α : Type) [Sized α] where
+  IdealT : Type -- Can split off `IdealT` to allow e.g. `Bool` being ideal without prime, I guess
+  toRepresents : IdealT → Vector (ZMod p) |α|
+
+export Convertible (toRepresents IdealT)
+
+structure Converts {p : ℕ}
+  {α : Type} [Sized α] [φ : Convertible p α]
   (varStore : VarStore p)
   (σ : HashConsSt p)
   (numAlloc : ℕ)
-  (exprs : Vector ExprRef k)
-  (val : α)
+  (exprs : Vector ExprRef |α|)
+  (val : IdealT p α)
 : Prop where
-  varSet_wf : ∀ (i : Fin k), ⦃exprs[i], σ⦄.varSet_wellFormed numAlloc
-  expr_wf   : ∀ (i : Fin k), ⦃exprs[i], σ⦄.wellFormed
-  value_eq  : ∀ (i : Fin k), [varStore|⦃exprs[i], σ⦄] = .some (conversion val)[i]
+  varSet_wf : ∀ (i : Fin |α|), ⦃exprs[i], σ⦄.varSet_wellFormed numAlloc
+  expr_wf   : ∀ (i : Fin |α|), ⦃exprs[i], σ⦄.wellFormed
+  value_eq  : ∀ (i : Fin |α|), [varStore|⦃exprs[i], σ⦄] = .some (toRepresents val)[i]
 
-structure Converts' {p : ℕ} {α : Type}
+structure Converts' {p : ℕ}
+  {α : Type}
   (conversion : α → List (ZMod p))
   (varStore : VarStore p)
   (σ : HashConsSt p)
@@ -30,59 +41,107 @@ structure Converts' {p : ℕ} {α : Type}
   expr_wf   : ∀ (i : Fin exprs.length), ⦃exprs[i], σ⦄.wellFormed
   value_eq  : ∀ (i : Fin exprs.length), [varStore|⦃exprs[i], σ⦄] = .some ((conversion val)[i])
 
--- structure HasSpec {p} {idealT} {representsT} (action : ClapM p representsT) where
---   spec : idealT
---   converts : Converts k conversion varStore σ numAlloc exprs spec
+@[aesop unsafe apply, grind .]
+lemma converts_of_converts' {p}
+  {α} [Sized α][Convertible p α]
+  {varStore : VarStore p} {σ : HashConsSt p} {numAlloc : ℕ}
+  {exprs : Vector ExprRef |α|} {val : IdealT p α}
+  {conversionList : IdealT p α → List (ZMod p)}
+  (h : Converts' conversionList varStore σ numAlloc exprs.toList val) 
+  (h_conversion :
+    ∀ i : Fin |α|,
+      (conversionList val)[i]'(by grind [cases Converts']) = (toRepresents val)[i]) :
+  Converts varStore σ numAlloc exprs val := by
+  rcases h with ⟨h₁, h₂, h₃, h₄⟩
+  rw! (castMode := .all) [show exprs.toList.length = |α| by aesop] at h₁ h₂ h₃ h₄
+  constructor <;> aesop (add safe (by grind))
+
+section OfDubiousWorth
 
 /-
-isZero.hasSpec a := {
-  spec := a == 0
-  converts : FB.ConvertsM (isZero a) spec
-}
-
-(a >>= f).spec = something
-
+Typeclasses make these awkward.
 -/
+
+@[aesop unsafe apply, grind .]
+lemma converts'_of_converts {p}
+  {α} [Sized α] [Convertible p α]
+  {varStore : VarStore p} {σ : HashConsSt p} {numAlloc : ℕ}
+  {exprs : Vector ExprRef |α|} {val : IdealT p α}
+  {conversionList : IdealT p α → List (ZMod p)}
+  (h_len : (conversionList val).length = |α|)
+  (h : Converts varStore σ numAlloc exprs val)
+  (h_conversion : ∀ i : Fin |α|, (conversionList val)[i] = (toRepresents val)[i]) :
+  Converts' conversionList varStore σ numAlloc exprs.toList val := by
+  rcases h with ⟨h₁, h₂, h₃⟩
+  constructor
+  all_goals
+    try intros i
+        rcases i with ⟨i, hi⟩
+    specialize_all (⟨i, by grind⟩ : Fin |α|)
+    aesop (add safe (by grind))
+
+@[grind .]
+lemma converts_iff_converts' {p}
+  {α} [Sized α] [Convertible p α]
+  {varStore : VarStore p} {σ : HashConsSt p} {numAlloc : ℕ}
+  {exprs : Vector ExprRef |α|} {val : IdealT p α}
+  {conversionList : IdealT p α → List (ZMod p)}
+  (h_len : (conversionList val).length = |α|)
+  (h_conversion : ∀ i : Fin |α|, (conversionList val)[i] = (toRepresents val)[i]) :
+  Converts varStore σ numAlloc exprs val ↔
+  Converts' conversionList varStore σ numAlloc exprs.toList val :=
+  ⟨
+    fun h ↦ converts'_of_converts h_len h h_conversion,
+    fun h ↦ converts_of_converts' h h_conversion
+  ⟩
+  
+end OfDubiousWorth
 
 section Lemmas
 
 variable
   {p k : ℕ}
   {α : Type}
-  {conversion : α → Vector (ZMod p) k}
+  {β : Type} [Sized β] [Convertible p β]
+  {conversionVec : β → Vector (ZMod p) |β|}
+  {conversionList : α  → List (ZMod p)}
+  {exprsVec : Vector ExprRef |β|}
+  {exprsList : List ExprRef}
+  {valVec : IdealT p β}
+  {valList : α}
   {Γ : VarStore p}
   {σ : HashConsSt p}
   {numAlloc : ℕ}
-  {exprs : Vector ExprRef k}
-  {val : α}
   {x : ZMod p}
-  {action : ClapM p α}
+  {actionList : ClapM p α}
+  {actionVec : ClapM p β}
   {circuit : Circuit}
 
-lemma converts_of_converts_eq
-  {val₁ : α} (val₂ : α)
+@[grind .]
+lemma coverts_of_converts_eq {val₁ val₂}
   (h : val₁ = val₂)
 :
-  Converts k conversion Γ σ numAlloc exprs val₁ ↔
-  Converts k conversion Γ σ numAlloc exprs val₂
+  Converts Γ σ numAlloc exprsVec val₁ ↔
+  Converts Γ σ numAlloc exprsVec val₂
 := by
   grind
 
 @[aesop unsafe]
 lemma isSome_eval_of_isSome_toIdeal
-  (h : Converts k conversion Γ σ numAlloc exprs val)
+  (h : Converts Γ σ numAlloc exprsVec valVec)
 :
-  ∀ i : Fin k, [Γ, σ|exprs[i]].isSome = true
+  ∀ i : Fin |β|, [Γ, σ|exprsVec[i]].isSome = true
 := fun i ↦ Option.isSome_iff_exists.2 ⟨_, h.value_eq i⟩
 
+@[aesop unsafe]
 lemma eval_varStore_eval_eq_some
-  {β}
-  {action : ClapM p β}
-  (h₁ : Converts k conversion Γ σ numAlloc exprs val)
-  (h₂ : action.hashConsState_wellFormed numAlloc σ)
+  (h₁ : Converts Γ σ numAlloc exprsVec valVec)
+  (h₂ : actionVec.hashConsState_wellFormed numAlloc σ)
 :
-  letI varStore' := [Γ, action.getHashConsState numAlloc σ, numAlloc|circuit]ₑ.varStore
-  ∀ i : Fin k, [varStore'|⦃exprs[i], action.getHashConsState numAlloc σ⦄] = some (conversion val)[i]
+  letI varStore' := [Γ, actionVec.getHashConsState numAlloc σ, numAlloc|circuit]ₑ.varStore
+  ∀ i : Fin |β|,
+    [varStore'|⦃exprsVec[i], actionVec.getHashConsState numAlloc σ⦄] =
+    some (toRepresents valVec)[i]
 := by
   intros i
   rcases circuit with ⟨l⟩
@@ -96,7 +155,7 @@ lemma eval_varStore_eval_eq_some
       apply eval_eq_of_varStore_eq_at_varSet
       . grind [Converts]
       . intro v h_v
-        set vashtorr := [unconstrained[numAlloc][Γ], action.getHashConsState numAlloc σ|hd]ₛ.varStore
+        set vashtorr := [unconstrained[numAlloc][Γ], actionVec.getHashConsState numAlloc σ|hd]ₛ.varStore
         rewrite [Circuit.getElem?_eval_eq_getElem?_of_lt (by grind [Converts])]
         rewrite [Circuit.getElem?_eval_eq_getElem?_of_lt (by grind [Converts])]
         choose k vec h_vec using @EvalSt.exists_varStore_step_eq_insertMany
@@ -105,19 +164,15 @@ lemma eval_varStore_eval_eq_some
         grind [Converts]
 
 lemma eval_varStore_eval_eq_some'
-  {β}
-  {conversion : α → List (ZMod p)}
-  {exprs : List ExprRef}
-  {action : ClapM p β}
-  (h₁ : Converts' conversion Γ σ numAlloc exprs val)
-  (h₂ : action.hashConsState_wellFormed numAlloc σ)
+  (h₁ : Converts' conversionList Γ σ numAlloc exprsList valList)
+  (h₂ : actionList.hashConsState_wellFormed numAlloc σ)
 :
-  letI varStore' := [Γ, action.getHashConsState numAlloc σ, numAlloc|circuit]ₑ.varStore
-  ∀ i : Fin exprs.length,
-    [varStore'|⦃exprs[i], action.getHashConsState numAlloc σ⦄] =
-    some ((conversion val)[i]'(by grind [cases Converts']))
+  letI varStore' := [Γ, actionList.getHashConsState numAlloc σ, numAlloc|circuit]ₑ.varStore
+  ∀ i : Fin exprsList.length,
+    [varStore'|⦃exprsList[i], actionList.getHashConsState numAlloc σ⦄] =
+    some ((conversionList valList)[i]'(by grind [cases Converts']))
 := by
-  intros i
+  intros i  
   rcases circuit with ⟨l⟩
   induction' eq : l.length with len ih generalizing l
   · rcases l <;> grind [Converts']
@@ -129,7 +184,7 @@ lemma eval_varStore_eval_eq_some'
       apply eval_eq_of_varStore_eq_at_varSet
       . grind [Converts']
       . intro v h_v
-        set vashtorr := [unconstrained[numAlloc][Γ], action.getHashConsState numAlloc σ|hd]ₛ.varStore
+        set vashtorr := [unconstrained[numAlloc][Γ], actionList.getHashConsState numAlloc σ|hd]ₛ.varStore
         rewrite [Circuit.getElem?_eval_eq_getElem?_of_lt (by grind [Converts'])]
         rewrite [Circuit.getElem?_eval_eq_getElem?_of_lt (by grind [Converts'])]
         choose k vec h_vec using @EvalSt.exists_varStore_step_eq_insertMany
@@ -138,17 +193,13 @@ lemma eval_varStore_eval_eq_some'
         grind [Converts']
 
 lemma toIdeal_run_of_toIdeal
-  {β}
-  (action : ClapM p β)
-  (h_a_wf : action.wellFormed numAlloc Γ σ)
-  (h : Converts k conversion Γ σ numAlloc exprs val) :
-  Converts k
-           conversion
-           (action.getVarStore Γ numAlloc σ)
-           (action.getHashConsState numAlloc σ)
-           (action.getNumAlloc numAlloc σ)
-           exprs
-           val := by
+  (h_a_wf : actionVec.wellFormed numAlloc Γ σ)
+  (h : Converts Γ σ numAlloc exprsVec valVec) :
+  Converts (actionVec.getVarStore Γ numAlloc σ)
+           (actionVec.getHashConsState numAlloc σ)
+           (actionVec.getNumAlloc numAlloc σ)
+           exprsVec
+           valVec := by
   rcases h with ⟨h₁, h₂, h₃⟩
   constructor
   · grind [=Expr.varSet_wellFormed]
@@ -156,141 +207,10 @@ lemma toIdeal_run_of_toIdeal
   · rcases h_a_wf with ⟨⟨h₄, h₅⟩, ⟨h₆, h₇⟩⟩
     intro i
     unfold ClapM.getVarStore
-    rw [eval_varStore_eval_eq_some (conversion := conversion) (val := val)]
+    rw [eval_varStore_eval_eq_some] -- a-HA!
     . constructor <;> assumption
     . assumption
 
 end Lemmas
 
 end Clap
-
--- structure Convert.toIdeal (varStore : VarStore p)
---                           (σ : HashConsSt p)
---                           (numAlloc : ℕ)
---                           (result : F)
---                           (x : ZMod p) : Prop where
---   varSet_wf : ⦃result, σ⦄.varSet_wellFormed numAlloc
---   expr_wf   : ⦃result, σ⦄.wellFormed
---   value_eq  : [varStore, σ|result] = .some x
-
--- structure _root_.Clap.Lang.FB.Convert.toIdeal (varStore : VarStore p)
---                                               (σ : HashConsSt p)
---                                               (numAlloc : ℕ)
---                                               (result : FB)
---                                               (x : Bool) : Prop where
---   varSet_wf : ⦃result, σ⦄.varSet_wellFormed numAlloc
---   expr_wf   : ⦃result, σ⦄.wellFormed
---   value_eq  : [varStore, σ|result] = .some (if x then 1 else 0)
-
--- structure _root_.Clap.Lang.FArray.Convert.toIdeal (varStore : VarStore p)
---                                                   (σ : HashConsSt p)
---                                                   (numAlloc : ℕ)
---                                                   {k : ℕ}
---                                                   (result : FArray k)
---                                                   (x : Vector Bool k) : Prop where
---   varSet_wf : ∀ elem ∈ result, ⦃elem, σ⦄.varSet_wellFormed numAlloc
---   expr_wf   : ∀ elem ∈ result, ⦃elem, σ⦄.wellFormed
---   value_eq  : ∀ (i : Fin k), [varStore, σ|result[i]] = .some (if x[i] then 1 else 0)
-
-
-
-
-
-
-
-
-
-
-
-
-
-
-
-
-
-
-
-
-
-
-
-
-
-
-
-
-
-
-
-
-
-
-
--- import Clap.eDSLState.IsValid
-
--- namespace Clap
-
--- class Convert (p : ℕ) (representsT idealT : Type) extends IsValid p representsT where
---   toIdeal : (VarStore p) → (HashConsSt p) → representsT → Option idealT
---   toRepresents : idealT → HashConsM p representsT
---   isValid_iff_isSome_toIdeal :
---     ∀ (varStore : VarStore p) (σ : HashConsSt p) (x : representsT),
---       isValid varStore σ x ↔ (toIdeal varStore σ x).isSome
---   toIdeal_toRepresents :
---     ∀ (varStore : VarStore p) (σ : HashConsSt p) (x : idealT),
---       toIdeal varStore ((toRepresents x).getHashConsState σ) ((toRepresents x).getResult σ) = .some x
-
--- @[simp, grind =]
--- lemma Convert.toRepresents_toIdeal
---   {p : ℕ}
---   {representsT idealT : Type}
---   [inst: Convert p representsT idealT]
---   {varStore : VarStore p}
---   {σ : HashConsSt p}
---   {x : representsT}
---   (h : IsValid.isValid varStore σ x)
--- :
---   toIdeal (representsT := representsT) (idealT := idealT) varStore σ
---     ((toRepresents (representsT := representsT) ((toIdeal (idealT := idealT) varStore σ x).get ((isValid_iff_isSome_toIdeal varStore σ x).mp h))).getResult σ) =
---   inst.toIdeal varStore σ x
--- := by
---   have := inst.toIdeal_toRepresents
---   simp [HashConsM.getHashConsState, HashConsM.getResult] at this ⊢
-
---   simp [inst.toIdeal_toRepresents]
-
--- instance {p : ℕ} : Convert p Unit Unit where
---   isValid := fun _ _ _ ↦ True
---   toIdeal _ x := .some x
---   toRepresents x := x
---   isValid_iff_isSome_toIdeal _ _ := by grind
---   toIdeal_toRepresents _ _ := by grind
-
--- @[simp, grind .]
--- lemma isValid_iff_isSome_toIdeal {p} {α β : Type} [Convert p α β]
---   {varStore : VarStore p} {σ : HashConsSt p} {x : α}
--- :
---   (Convert.toIdeal (idealT := β) varStore x).isSome ↔
---   IsValid.isValid varStore σ x
--- := by
---   aesop (add safe cases Convert)
-
--- @[grind .]
--- lemma isValid_of_toIdeal_eq_some {p} {α β : Type} [Convert p α β]
---   {varStore : VarStore p} {x : α} {b : β}
---   (h : (Convert.toIdeal (idealT := β) varStore x) = .some b)
--- :
---   IsValid.isValid varStore x
--- := by
---   have := Option.isSome_of_eq_some h
---   grind
-
--- @[simp, grind .]
--- lemma toIdealtoRepresents_of_convert {p} {α β : Type} [Convert p α β]
---   {varStore : VarStore p} {x : β}
--- :
---   Convert.toIdeal (representsT := α) varStore (Convert.toRepresents p x) = .some x
--- := by
---   aesop (add safe cases Convert)
-
--- end Clap
